steel/Zeta.Steel.BitUtils.fsti
@@ -13,3 +13,12 @@ val bitvec_of_u256_inj (i j:_)
              i == j)
     [SMTPat (bitvec_of_u256 i);
      SMTPat (bitvec_of_u256 j)]
+
+let zero256: T.hash_value =
+  let open T in
+  let z = FStar.UInt64.zero in
+  { v3 = z; v2 = z; v1 = z ; v0 = z }
+
+val related_zero (_:unit)
+  : Lemma (bitvec_of_u256 zero256 ==
+           FStar.BitVector.zero_vec #256)
